@prefix : <http://www.isfla.org/gam-sfg-mm#> .
@prefix gam: <http://www.isfla.org/gam-core#> .
@prefix olo: <http://purl.org/ontology/olo/core#> .
@prefix owl: <http://www.w3.org/2002/07/owl#> .
@prefix rdf: <http://www.w3.org/1999/02/22-rdf-syntax-ns#> .
@prefix xml: <http://www.w3.org/XML/1998/namespace> .
@prefix xsd: <http://www.w3.org/2001/XMLSchema#> .
@prefix rdfs: <http://www.w3.org/2000/01/rdf-schema#> .
@base <http://www.isfla.org/gam-sfg-mm> .

<http://www.isfla.org/gam-sfg-mm> rdf:type owl:Ontology ;
                                  
                                  rdfs:label "Generalised Annotation Model: Systemic Functional Grammar"^^rdfs:Literal ;
                                  
                                  owl:versionInfo "1.0"^^rdfs:Literal ;
                                  
                                  rdfs:comment "Contains Integrity Constratints corresponding to the SFG meta model (the model of theory of grammar)"^^rdfs:Literal ;
                                  
                                  owl:imports <http://www.isfla.org/gam-core/1.0> ;
                                  
                                  owl:versionIRI <http://www.isfla.org/gam-sfg-mm/1.0> .


#################################################################
#
#    Object Properties
#
#################################################################


###  http://www.isfla.org/gam-core#composes

gam:composes rdfs:range gam:Composite ;
             
             rdfs:domain gam:FunctionalElement .



###  http://www.isfla.org/gam-core#constituencyRelation

gam:constituencyRelation rdf:type owl:TransitiveProperty .



###  http://www.isfla.org/gam-core#constitutes

gam:constitutes rdf:type owl:TransitiveProperty ;
                
                rdfs:comment """relationship between lower constituent to a parent constituent.
in SFG this is an indirect relationship going through a FunctionalElement by a chain of two other relations fills + composes || expounds + composes"""^^rdfs:Literal ;
                
                rdfs:range gam:Composite ;
                
                rdfs:domain gam:Unit ;
                
                owl:propertyChainAxiom ( gam:fills
                                         gam:composes
                                       ) ,
                                       ( gam:expounds
                                         gam:composes
                                       ) .



###  http://www.isfla.org/gam-core#expounds

gam:expounds rdfs:range gam:FunctionalElement ;
             
             rdfs:domain gam:LexicalItem .



###  http://www.isfla.org/gam-core#extends

gam:extends rdfs:domain gam:FunctionalElement ;
            
            rdfs:range gam:FunctionalElement .



###  http://www.isfla.org/gam-core#fills

gam:fills rdfs:domain gam:Composite ;
          
          rdfs:range gam:FunctionalElement .



###  http://www.isfla.org/gam-core#hasConstituent

gam:hasConstituent rdf:type owl:TransitiveProperty ;
                   
                   rdfs:comment """constituency relation links two units together as a chain of two properties leading via a functional element. 
constituency relation can be acheived either through isComposedOf + isExpoubndedBy sequence of relations OR by isComposedOf + isFilledBy sequence of relations"""^^rdfs:Literal ;
                   
                   rdfs:domain gam:Composite ;
                   
                   rdfs:range gam:Unit ;
                   
                   owl:propertyChainAxiom ( gam:isComposedOf
                                            gam:isFilledBy
                                          ) ,
                                          ( gam:isComposedOf
                                            gam:isExpoundedBy
                                          ) .



###  http://www.isfla.org/gam-core#isComposedOf

gam:isComposedOf rdfs:domain gam:Composite ;
                 
                 rdfs:range gam:FunctionalElement .



###  http://www.isfla.org/gam-core#isExpoundedBy

gam:isExpoundedBy rdfs:domain gam:FunctionalElement ;
                  
                  rdfs:range gam:LexicalItem .



###  http://www.isfla.org/gam-core#isFilledBy

gam:isFilledBy rdfs:range gam:Composite ;
               
               rdfs:domain gam:FunctionalElement .





#################################################################
#
#    Classes
#
#################################################################


###  http://www.isfla.org/gam-core#Composite

gam:Composite rdfs:subClassOf [ rdf:type owl:Restriction ;
                                owl:onProperty gam:isComposedOf ;
                                owl:onClass gam:FunctionalElement ;
                                owl:minQualifiedCardinality "1"^^xsd:nonNegativeInteger
                              ] ,
                              [ rdf:type owl:Restriction ;
                                owl:onProperty gam:hasConstituent ;
                                owl:onClass gam:Unit ;
                                owl:minQualifiedCardinality "1"^^xsd:nonNegativeInteger
                              ] .



###  http://www.isfla.org/gam-core#FunctionalElement

gam:FunctionalElement rdfs:subClassOf [ rdf:type owl:Restriction ;
                                        owl:onProperty gam:composes ;
                                        owl:onClass gam:Composite ;
                                        owl:qualifiedCardinality "1"^^xsd:nonNegativeInteger
                                      ] ,
                                      [ rdf:type owl:Class ;
                                        owl:unionOf ( [ rdf:type owl:Restriction ;
                                                        owl:onProperty gam:isExpoundedBy ;
                                                        owl:onClass gam:LexicalItem ;
                                                        owl:qualifiedCardinality "1"^^xsd:nonNegativeInteger
                                                      ]
                                                      [ rdf:type owl:Restriction ;
                                                        owl:onProperty gam:isFilledBy ;
                                                        owl:onClass gam:Composite ;
                                                        owl:qualifiedCardinality "1"^^xsd:nonNegativeInteger
                                                      ]
                                                    )
                                      ] ;
                      
                      rdfs:comment """in SFL model FunctionalElement is 
* an instance of Functional element defines the structure of exactly one unit. In other words the same element instance cannot define the functional structure  of multiple units
* filled by exactly one Unit or expounded by exactly one Lexical Item (this constraint does not exist in official Cardiff Grammar where conjuncted units fill the same functional element)"""^^rdfs:Literal .



###  http://www.isfla.org/gam-core#LinguisticMetafunction

gam:LinguisticMetafunction owl:disjointUnionOf ( :Experiential
                                                 :Interpersonal
                                                 :Logical
                                                 :Textual
                                               ) .



###  http://www.isfla.org/gam-sfg-mm#Experiential

:Experiential rdf:type owl:Class ;
              
              rdfs:subClassOf gam:LinguisticMetafunction .



###  http://www.isfla.org/gam-sfg-mm#Interpersonal

:Interpersonal rdf:type owl:Class ;
               
               rdfs:subClassOf gam:LinguisticMetafunction .



###  http://www.isfla.org/gam-sfg-mm#Logical

:Logical rdf:type owl:Class ;
         
         rdfs:subClassOf gam:LinguisticMetafunction .



###  http://www.isfla.org/gam-sfg-mm#Textual

:Textual rdf:type owl:Class ;
         
         rdfs:subClassOf gam:LinguisticMetafunction .





#################################################################
#
#    Annotations
#
#################################################################


gam:linearOrderRelation rdfs:comment """in SFG to be used 
* eventually for defining the relative order of functional elements within a grammatical unit structures.
* always for instances of lexical items"""^^rdfs:Literal .




###  Generated by the OWL API (version 3.5.1) http://owlapi.sourceforge.net

